src/program_proof/memkv/memkv_shard_start_proof.v
@@ -9,7 +9,7 @@ Section memkv_shard_start_proof.
 Context `{!heapG Σ, rpcG Σ ShardReplyC, rpcregG Σ, kvMapG Σ}.
 
 Lemma wp_MemKVShardServer__Start (s:loc) (host : u64) γ :
-handlers_dom host γ.(urpc_gn) {[ U64 0; U64 1; U64 2; U64 3; U64 4; U64 5 ]} -∗
+handlers_dom γ.(urpc_gn) {[ U64 0; U64 1; U64 2; U64 3; U64 4; U64 5 ]} -∗
 is_shard_server host γ -∗
 is_MemKVShardServer s γ -∗
   {{{
